theories/helpers.v
@@ -4,5 +4,9 @@ Section slice.
   Context {A : Type}.
   Implicit Types l : list A.
 
-  Definition slice l a b := take b (drop a l).
+  (* k elements starting from i-th *)
+  Definition slice l i k := take k (drop i l).
+
+  Lemma slice_0 l i : slice l i 0 = [].
+  Proof. auto. Qed.
 End slice.
